Done BT_def

examples/lambda/completeness/boehm_treeScript.sml
@@ -8,23 +8,14 @@ open HolKernel boolLib Parse bossLib;
 open optionTheory arithmeticTheory pred_setTheory listTheory llistTheory
      ltreeTheory pathTheory hurdUtils;
 
-(* theories in ../basics *)
-open binderLib termTheory appFOLDLTheory;
-
-(* theories in ../barendregt *)
-open chap2Theory chap3Theory head_reductionTheory standardisationTheory
-     solvableTheory;
-
-(* theories in ../other-models *)
-open pure_dBTheory;
+open binderLib termTheory appFOLDLTheory chap2Theory chap3Theory
+     head_reductionTheory standardisationTheory solvableTheory pure_dBTheory;
 
 val _ = new_theory "boehm_tree";
 
-(*---------------------------------------------------------------------------*
- * Principle Head Normal Forms (phnf)
- *---------------------------------------------------------------------------*)
+val o_DEF = combinTheory.o_DEF;
 
- (* Definition 8.3.20 [1, p.177]
+(* Definition 8.3.20 [1, p.177]
 
    A term may have several hnf's, e.g. if any of its hnf can still do beta
    reductions, after such reductions the term is still an hnf by definition.
@@ -32,13 +23,13 @@ val _ = new_theory "boehm_tree";
    hnf, which is used for defining Boehm trees.
  *)
 Definition phnf_def :
-    phnf (M :term) = last (head_reduction_path M)
+    phnf = last o head_reduction_path
 End
 
 Theorem solvable_phnf :
     !M. solvable M ==> hnf (phnf M)
 Proof
-    rw [solvable_iff_has_hnf, phnf_def, head_reduction_path_def, corollary11_4_8]
+    rw [o_DEF, solvable_iff_has_hnf, phnf_def, head_reduction_path_def, corollary11_4_8]
 QED
 
 (* NOTE: this function was impossible for “:term” *)
@@ -204,34 +195,21 @@ Proof
  >> rw []
 QED
 
-(* Now applying ltree_unfold to build the Boehm Tree *)
-
-(*
-Definition BT0_def :
-   (BT0 (M :term) ([] :num list) = if unsolvable M then NONE
-                                  else ARB) /\
-   (BT0 (M :term) (k::ks) = if unsolvable M then ARB else
-                           ARB)
+(* The needed unfolding function for ltree_unfold for Boehm Tree *)
+Definition BT_generator_def :
+    BT_generator (M :pdb) = if solvable (toTerm M) then
+                               (SOME (dABSi (dABSn M) (dV (dVn M))),
+                                fromList (dAPPl M))
+                            else
+                               (NONE, LNIL)
 End
 
-(* NOTE: “hnf_of” is undefined
-   (cf. normal_orderTheory.bnf_of_def or head_reductionTheory)
- *)
+(* So this is BT(M) *)
 Definition BT_def :
-   BT M = if unsolvable M then (\s. NONE)
-          else BT0 (hnf_of M)
+    BT (M :pdb) = ltree_unfold BT_generator M
 End
 
-(* When M is solvable and has principal hnf *)
-Definition BTe_def :
-   (BTe (M :term) ([] :num list) =
-        if has_hnf M then (SOME (LAMl vs (VAR y)), LENGTH Ms)
-        else (NONE, 0)) /\
-   (BTe M (k::xs) =
-        if has_hnf M then BTe [EL k Ms] xs
-        else (NONE, 0)
-End
-*)
+Type boehm_tree[pp] = “:pdb option ltree”
 
 val _ = export_theory ();
 val _ = html_theory "boehm_tree";
